@prefix cov: <http://kdmg.dii.univpm.it/datasets/covid19italy/> .
@prefix covt: <http://kdmg.dii.univpm.it/datasets/covid19italy/terms> .
@prefix dbr: <http://dbpedia.org/resource/> .
@prefix qb: <http://purl.org/linked-data/cube#> .
@prefix xsd: <http://www.w3.org/2001/XMLSchema#> .

#Definition of measures

covt:Total_Hospitalised_Patients_With_Symptoms a kpi:Indicator;
 rdfs:label "Total hospitalized patients with symptoms";
 rdfs:comment "Current total number of cases hospitalized with symptoms on the reference time".

covt:Total_Intensive_Care a kpi:Indicator;
 rdfs:label "Total intensive care";
 rdfs:comment "Current total number of cases hospitalized requiring intensive care on the reference time".

covt:Total_Hospitalised_Patients a kpi:Indicator;
 rdfs:label "Total hospitalised patiens";
 rdfs:comment "Current total number of positive patients hospitalised on the reference time";
 kpi:hasFormula [
		kpi:hasFunction om:plus;
                kpi:hasArgument
			[kpi:hasArgumentPosition 1;
			 kpi:hasArgumentName "addend";
			 kpi:hasArgumentValue covt:Total_Hospitalised_Patients_With_Symptoms];
                kpi:hasArgument
			[kpi:hasArgumentPosition 2;
			 kpi:hasArgumentName "addend";
			 kpi:hasArgumentValue covt:Total_Intensive_Care]
		].

covt:Total_Home_Confinement a kpi:Indicator;
 rdfs:label "Total home confinement";
 rdfs:comment "Current total number of cases in home confinement on the reference time".

covt:Total_Positive_Cases a kpi:Indicator;
 rdfs:label "Total positive cases";
 rdfs:comment "Current total number of positive cases on the reference time";
  kpi:hasFormula [
		kpi:hasFunction om:plus;
                kpi:hasArgument
			[kpi:hasArgumentPosition 1;
			 kpi:hasArgumentName "addend";
			 kpi:hasArgumentValue covt:Total_Hospitalised_Patients];
                kpi:hasArgument
			[kpi:hasArgumentPosition 2;
			 kpi:hasArgumentName "addend";
			 kpi:hasArgumentValue covt:Total_Home_Confinement]
		].

covt:Variation_Total_Positive_Cases a kpi:Indicator;
 rdfs:label "Variation total positive cases";
 rdfs:comment "Variation of the current number of total positive cases with respect to the previous measurement".

covt:New_Cases a kpi:Indicator;
 rdfs:label "New cases";
 rdfs:comment "Number of new cases".

covt:Total_Recovered a kpi:Indicator;
 rdfs:label "Total recovered";
 rdfs:comment "Current total number of recovered cases on the reference time".

covt:Total_Deaths a kpi:Indicator;
 rdfs:label "Total deaths";
 rdfs:comment "Current total number of deaths on the reference time".

covt:Total_Cases a kpi:Indicator;
 rdfs:label "Total cases";
 rdfs:comment "Current total number of cases on the reference time";
  kpi:hasFormula [
		kpi:hasFunction om:plus;
                kpi:hasArgument
			[kpi:hasArgumentPosition 1;
			 kpi:hasArgumentName "addend";
			 kpi:hasArgumentValue cov:Total_Positive_Cases];
                kpi:hasArgument
			[kpi:hasArgumentPosition 2;
			 kpi:hasArgumentName "addend";
			 kpi:hasArgumentValue [
				kpi:hasFunction om:plus;
                		kpi:hasArgument
					[kpi:hasArgumentPosition 1;
					 kpi:hasArgumentName "addend";
					 kpi:hasArgumentValue cov:Total_Recovered],
					[kpi:hasArgumentPosition 2;
					 kpi:hasArgumentName "addend";
					 kpi:hasArgumentValue cov:Total_Deaths]
			        ]
                       ]
  ]. 


covt:Total_Tests_Performed a kpi:Indicator;
 rdfs:label "Total tests";
 rdfs:comment "Current total number of tests on the reference time".

covt:Total_Cases_Tested a kpi:Indicator;
 rdfs:label "Total number of cases tested";
 rdfs:comment "Current total number of cases tested on the reference time".


#Definition of notes

covt:Note a rdfs:Class;
	rdfs:comment "A note attached to an observation."^^xsd:string.

covt:PartialDataNote rdfs:subClassOf covt:Note;
	rdfs:comment "A note declaring that data is partial."^^xsd:string.

covt:NoDataNote rdfs:subClassOf covt:Note.
	rdfs:comment "A note declaring that data is not available."^^xsd:string.

covt:DataCorrectionNote rdfs:subClassOf covt:Note.
	rdfs:comment "A note declaring a data correction."^^xsd:string.

covt:noticeDescription rdfs:subPropertyOf rdf:Property;
	rdfs:domain covt:Note;
	rdfs:range rdfs:Literal.

covt:otherInformation rdfs:subPropertyOf rdf:Property;
	rdfs:domain covt:Note;
	rdfs:range rdfs:Literal.

covt:note rdfs:subPropertyOf rdf:Property;
	rdfs:domain qb:Observation;
	rdfs:range covt:Note.


